theories/Frontend/Cst.v
@@ -1,0 +1,19 @@
+From Coq Require Import String.
+
+(** * Concrete Syntax Tree *)
+Inductive obj : Set :=
+| cst_typ : nat -> obj
+| cst_nat : obj
+| cst_zero : obj
+| cst_succ : obj -> obj
+| cst_natrec : obj -> string -> obj -> obj -> string -> string -> obj -> obj
+| cst_pi : string -> obj -> obj -> obj
+| cst_fn : string -> obj -> obj -> obj
+| cst_app : obj -> obj -> obj
+| cst_prop_eq : obj -> obj -> obj -> obj
+| cst_refl : obj -> obj -> obj
+| cst_eqrec : obj ->                            (** A : eq domain type *)
+              string -> string -> string -> obj -> (** x y (z : Eq A x y). M *)
+              string -> obj ->                   (** x. Pf : M[x/x, x/y, refl A x/z] *)
+              obj -> obj -> obj -> obj
+| cst_var : string -> obj.
